Experimenting

Constructors.v
@@ -2,6 +2,38 @@ From Elo Require Import Core.
 From Elo Require Import Definitions.
 From Elo Require Import Inversions.
 
+Class ConsMust (P : tm -> Prop) := {
+  cons_new   : forall t T,   P t          -> P <{new T t}>;
+  cons_load  : forall t,     P t          -> P <{*t}>;
+  cons_asg   : forall t1 t2, P t1 -> P t2 -> P <{t1 = t2}>;
+  cons_fun   : forall x T t, P t          -> P <{fn x T t}>;
+  cons_call  : forall t1 t2, P t1 -> P t2 -> P <{call t1 t2}>;
+  cons_seq   : forall t1 t2, P t1 -> P t2 -> P <{t1; t2}>;
+  cons_spawn : forall t,     P t          -> P <{spawn t}>;
+}.
+
+Class ConsUnit (P : tm -> Prop) := {
+  cons_unit : P <{unit}>;
+}.
+
+Class ConsNum (P : tm -> Prop) := {
+  cons_num : forall n,  P <{N n}>;
+}.
+
+Class ConsRef (P : tm -> Prop) := {
+  cons_ref : forall ad T,  P <{&ad :: T}>;
+}.
+
+Class ConsVar (P : tm -> Prop) := {
+  cons_var : forall x,  P <{var x}>;
+}.
+
+Ltac eauto_cons :=
+  eauto using cons_new, cons_load, cons_asg,
+              cons_fun, cons_call,
+              cons_seq,
+              cons_spawn.
+
 (* ------------------------------------------------------------------------- *)
 (* valid-addresses construction                                              *)
 (* ------------------------------------------------------------------------- *)
@@ -70,6 +102,28 @@ Proof. solve_vad_construction. Qed.
   vad_var vad_fun vad_call vad_seq vad_spawn
   : vad.
 
+#[export] Instance ConsVAD : forall m, ConsMust (valid_addresses m) := {
+  cons_new   := vad_new m;
+  cons_load  := vad_load m;
+  cons_asg   := vad_asg m;
+  cons_fun   := vad_fun m;
+  cons_call  := vad_call m;
+  cons_seq   := vad_seq m;
+  cons_spawn := vad_spawn m;
+}.
+
+#[export] Instance ConsVADUnit : forall m, ConsUnit (valid_addresses m) := {
+  cons_unit := vad_unit m;
+}.
+
+#[export] Instance ConsVADNum : forall m, ConsNum (valid_addresses m) := {
+  cons_num := vad_num m;
+}.
+
+#[export] Instance ConsVADVar : forall m, ConsVar (valid_addresses m) := {
+  cons_var := vad_var m;
+}.
+
 (* ------------------------------------------------------------------------- *)
 (* not-access constructors                                                   *)
 (* ------------------------------------------------------------------------- *)
@@ -109,6 +163,10 @@ Lemma nacc_asg : forall m t1 t2 ad,
   ~ access ad m <{t1 = t2}>.
 Proof. solve_nacc_construction. Qed.
 
+Lemma nacc_var : forall m x ad,
+  ~ access ad m <{var x}>.
+Proof. solve_nacc_construction. Qed.
+
 Lemma nacc_fun : forall m x Tx t ad,
   ~ access ad m t ->
   ~ access ad m <{fn x Tx t}>.
@@ -133,7 +191,7 @@ Proof. solve_nacc_construction. Qed.
 #[export] Hint Resolve
   nacc_unit nacc_num
   nacc_ref nacc_new nacc_load nacc_asg
-  nacc_fun nacc_call
+  nacc_var nacc_fun nacc_call
   nacc_seq
   nacc_spawn
   : acc.
